README.md
@@ -1,1 +1,15 @@
 # easycrypt-zk-code
+
+
+
+
+lemma nosmt modzMml: forall (m n d : int), m %% d * n %% d = m * n %% d.
+lemma nosmt modzMmr: forall (m n d : int), m * (n %% d) %% d = m * n %% d.
+lemma nosmt modzMm:
+  forall (m n d : int), m %% d * (n %% d) %% d = m * n %% d.
+lemma nosmt modzNm: forall (m d : int), (- m %% d) %% d = (-m) %% d.
+lemma nosmt mulz_modr:
+  forall (p m d : int), 0 < p => p * (m %% d) = p * m %% (p * d).
+lemma nosmt mulz_modl:
+  forall (p m d : int), 0 < p => m %% d * p = m * p %% (d * p).
+
